Carve out lemmas to StateTransition.thy

Isabelle/SafetyOracle.thy
@@ -1,6 +1,6 @@
 theory SafetyOracle
 
-imports Main CBCCasper ConsensusSafety
+imports Main CBCCasper StateTransition
 
 begin
 
@@ -103,78 +103,6 @@ fun (in Protocol) is_clique :: "(validator set * consensus_value_property * stat
 
 
 (* Section 7.3: Cliques Survive Messages from Validators Outside Clique *)
-
-(* Definition 7.17 *)
-abbreviation (in Protocol) minimal_transitions :: "(state * state) set"
-  where
-    "minimal_transitions \<equiv> {(\<sigma>, \<sigma>') | \<sigma> \<sigma>'. \<sigma> \<in> \<Sigma>t \<and> \<sigma>' \<in> \<Sigma>t \<and> is_future_state (\<sigma>', \<sigma>) \<and> \<sigma> \<noteq> \<sigma>'
-      \<and> (\<nexists> \<sigma>''. \<sigma>'' \<in> \<Sigma> \<and> is_future_state (\<sigma>'', \<sigma>) \<and> is_future_state (\<sigma>', \<sigma>'') \<and> \<sigma> \<noteq> \<sigma>'' \<and> \<sigma>'' \<noteq> \<sigma>')}"
-
-(* A minimal transition corresponds to receiving a single new message with justification drawn from the initial
-protocol state *)
-definition immediately_next_message where
-  "immediately_next_message = (\<lambda>(\<sigma>,m). justification m \<subseteq> \<sigma> \<and> m \<notin> \<sigma>)"
-
-lemma (in Protocol) message_cannot_justify_itself: "\<nexists>m. m \<in> M \<longrightarrow> m \<in> justification m"
-  sorry
-
-lemma (in Protocol) state_transition_by_immediately_next_message_induction: "\<forall>n\<ge>1. \<forall>\<sigma>\<in>\<Sigma>_i (V,C,\<epsilon>) n. \<forall>m\<in>M_i (V,C,\<epsilon>) n. immediately_next_message (\<sigma>,m) \<longrightarrow> \<sigma> \<union> {m} \<in> \<Sigma>_i (V,C,\<epsilon>) (n+1)"
-  apply (rule, rule, rule, rule, rule)
-proof-
-  fix n \<sigma> m
-  assume "1 \<le> n" "\<sigma> \<in> \<Sigma>_i (V, C, \<epsilon>) n" "m \<in> M_i (V, C, \<epsilon>) n" "immediately_next_message (\<sigma>, m)"
-
-  have "\<exists>n'. n = Suc n'"
-    using \<open>1 \<le> n\<close> old.nat.exhaust by auto
-  hence si: "\<Sigma>_i (V,C,\<epsilon>) n = {\<sigma> \<in> Pow (M_i (V,C,\<epsilon>) (n - 1)). \<forall> m. m \<in> \<sigma> \<longrightarrow> justification m \<subseteq> \<sigma>}"
-    by force
-
-  hence "\<Sigma>_i (V,C,\<epsilon>) (n+1) = {\<sigma> \<in> Pow (M_i (V,C,\<epsilon>) n). \<forall> m. m \<in> \<sigma> \<longrightarrow> justification m \<subseteq> \<sigma>}"
-    by force
-
-  have "justification m \<subseteq> \<sigma>"
-    using immediately_next_message_def
-    by (metis (no_types, lifting) \<open>immediately_next_message (\<sigma>, m)\<close> case_prod_conv)
-  hence "justification m \<subseteq> \<sigma> \<union> {m}"
-    by blast
-  moreover have "\<And>m'. m' \<in> \<sigma> \<Longrightarrow> justification m' \<subseteq> \<sigma>"
-    using \<open>\<sigma> \<in> \<Sigma>_i (V, C, \<epsilon>) n\<close> si by blast
-  hence"\<And>m'. m' \<in> \<sigma> \<Longrightarrow> justification m' \<subseteq> \<sigma> \<union> {m}"
-    by auto
-  ultimately have "\<And>m'. m' \<in> \<sigma> \<union> {m} \<Longrightarrow> justification m \<subseteq> \<sigma>"
-    using \<open>justification m \<subseteq> \<sigma>\<close> by blast
-
-  have "{m} \<in> Pow (M_i (V,C,\<epsilon>) n)"
-    using \<open>m \<in> M_i (V, C, \<epsilon>) n\<close> by auto
-  moreover have "\<sigma> \<in> Pow (M_i (V,C,\<epsilon>) (n-1))"
-    using \<open>\<sigma> \<in> \<Sigma>_i (V, C, \<epsilon>) n\<close> si by auto
-  hence "\<sigma> \<in> Pow (M_i (V,C,\<epsilon>) n)"
-    using Mi_monotonic
-    by (metis (full_types) PowD PowI Suc_eq_plus1 \<open>\<exists>n'. n = Suc n'\<close> diff_Suc_1 subset_iff)
-  ultimately have "\<sigma> \<union> {m} \<in> Pow (M_i (V,C,\<epsilon>) n)"
-    by blast
-
-  show "\<sigma> \<union> {m} \<in> \<Sigma>_i (V, C, \<epsilon>) (n + 1)"
-    using \<open>\<And>m'. m' \<in> \<sigma> \<Longrightarrow> justification m' \<subseteq> \<sigma> \<union> {m}\<close> \<open>\<sigma> \<union> {m} \<in> Pow (M_i (V, C, \<epsilon>) n)\<close> \<open>justification m \<subseteq> \<sigma> \<union> {m}\<close> by auto
-qed
-
-lemma (in Protocol) state_transition_by_immediately_next_message_at_n: "\<forall>\<sigma>\<in>\<Sigma>_i (V,C,\<epsilon>) n. \<forall>m\<in>M_i (V,C,\<epsilon>) n. immediately_next_message (\<sigma>,m) \<longrightarrow> \<sigma> \<union> {m} \<in> \<Sigma>_i (V,C,\<epsilon>) (n+1)"
-  apply (cases n)
-  apply auto[1]
-  using state_transition_by_immediately_next_message_induction
-  by (metis le_add1 plus_1_eq_Suc)
-
-lemma (in Protocol) state_differences_have_immediately_next_messages: 
-  "\<forall>\<sigma>\<in>\<Sigma>. \<forall>\<sigma>'\<in>\<Sigma>. is_future_state (\<sigma>', \<sigma>) \<and> \<sigma> \<noteq> \<sigma>' \<longrightarrow> (\<exists>m \<in> (\<sigma>'-\<sigma>). justification m \<subseteq> \<sigma>)"
-  oops  
-
-lemma (in Protocol) no_missing_message: "\<forall>\<sigma>\<in>\<Sigma>. \<forall>m\<in>\<sigma>. \<forall>m'\<in>justification m. m' \<in> \<sigma>"
-  using state_is_in_pow_M_i by fastforce
-
-lemma (in Protocol) minimal_transition_implies_recieving_a_single_message :
-  "\<forall> \<sigma> \<sigma>'. \<sigma> \<in> \<Sigma>t \<and> \<sigma>' \<in> \<Sigma>t
-  \<longrightarrow> (\<sigma>, \<sigma>') \<in> minimal_transitions  \<longrightarrow> is_singleton (\<sigma>'- \<sigma>)"
-  sorry
 
 (* Lemma 11: Minimal transitions do not change Later_From for any non-sender *)
 lemma (in Protocol) later_from_not_affected_by_minimal_transitions :
