Isabelle/LatestMessage.thy
@@ -73,13 +73,6 @@ lemma (in Protocol) monotonicity_of_justifications :
   "\<forall> m m' \<sigma>. m \<in> M \<and> \<sigma> \<in> \<Sigma> \<and> m' \<in> later (m, \<sigma>) \<longrightarrow> justification m \<subseteq> justification m'"
   using M_type state_is_in_pow_M_i by auto
 
-lemma (in Protocol) transitivity_of_justifications :
-  "\<forall> m1 m2 m3 \<sigma>. {m1, m2, m3} \<subseteq> \<sigma> \<and> \<sigma> \<in> \<Sigma> 
-  \<longrightarrow> m1 \<in> justification m2 \<and> m2 \<in> justification m3
-  \<longrightarrow> m1 \<in> justification m3"
-  by (meson M_type contra_subsetD insert_subset message_in_state_is_valid state_is_in_pow_M_i)
-
-
 (* Lemma 8 *)
 (* TODO *)
 
