Isabelle/StateTransition.thy
@@ -1,0 +1,91 @@
+theory StateTransition
+
+imports Main CBCCasper ConsensusSafety
+
+begin
+
+
+(* Definition 7.17 *)
+abbreviation (in Protocol) minimal_transitions :: "(state * state) set"
+  where
+    "minimal_transitions \<equiv> {(\<sigma>, \<sigma>') | \<sigma> \<sigma>'. \<sigma> \<in> \<Sigma>t \<and> \<sigma>' \<in> \<Sigma>t \<and> is_future_state (\<sigma>', \<sigma>) \<and> \<sigma> \<noteq> \<sigma>'
+      \<and> (\<nexists> \<sigma>''. \<sigma>'' \<in> \<Sigma> \<and> is_future_state (\<sigma>'', \<sigma>) \<and> is_future_state (\<sigma>', \<sigma>'') \<and> \<sigma> \<noteq> \<sigma>'' \<and> \<sigma>'' \<noteq> \<sigma>')}"
+
+(* A minimal transition corresponds to receiving a single new message with justification drawn from the initial
+protocol state *)
+definition immediately_next_message where
+  "immediately_next_message = (\<lambda>(\<sigma>,m). justification m \<subseteq> \<sigma> \<and> m \<notin> \<sigma>)"
+
+lemma (in Protocol) state_transition_by_immediately_next_message_induction: "\<forall>n\<ge>1. \<forall>\<sigma>\<in>\<Sigma>_i (V,C,\<epsilon>) n. \<forall>m\<in>M_i (V,C,\<epsilon>) n. immediately_next_message (\<sigma>,m) \<longrightarrow> \<sigma> \<union> {m} \<in> \<Sigma>_i (V,C,\<epsilon>) (n+1)"
+  apply (rule, rule, rule, rule, rule)
+proof-
+  fix n \<sigma> m
+  assume "1 \<le> n" "\<sigma> \<in> \<Sigma>_i (V, C, \<epsilon>) n" "m \<in> M_i (V, C, \<epsilon>) n" "immediately_next_message (\<sigma>, m)"
+
+  have "\<exists>n'. n = Suc n'"
+    using \<open>1 \<le> n\<close> old.nat.exhaust by auto
+  hence si: "\<Sigma>_i (V,C,\<epsilon>) n = {\<sigma> \<in> Pow (M_i (V,C,\<epsilon>) (n - 1)). \<forall> m. m \<in> \<sigma> \<longrightarrow> justification m \<subseteq> \<sigma>}"
+    by force
+
+  hence "\<Sigma>_i (V,C,\<epsilon>) (n+1) = {\<sigma> \<in> Pow (M_i (V,C,\<epsilon>) n). \<forall> m. m \<in> \<sigma> \<longrightarrow> justification m \<subseteq> \<sigma>}"
+    by force
+
+  have "justification m \<subseteq> \<sigma>"
+    using immediately_next_message_def
+    by (metis (no_types, lifting) \<open>immediately_next_message (\<sigma>, m)\<close> case_prod_conv)
+  hence "justification m \<subseteq> \<sigma> \<union> {m}"
+    by blast
+  moreover have "\<And>m'. m' \<in> \<sigma> \<Longrightarrow> justification m' \<subseteq> \<sigma>"
+    using \<open>\<sigma> \<in> \<Sigma>_i (V, C, \<epsilon>) n\<close> si by blast
+  hence"\<And>m'. m' \<in> \<sigma> \<Longrightarrow> justification m' \<subseteq> \<sigma> \<union> {m}"
+    by auto
+  ultimately have "\<And>m'. m' \<in> \<sigma> \<union> {m} \<Longrightarrow> justification m \<subseteq> \<sigma>"
+    using \<open>justification m \<subseteq> \<sigma>\<close> by blast
+
+  have "{m} \<in> Pow (M_i (V,C,\<epsilon>) n)"
+    using \<open>m \<in> M_i (V, C, \<epsilon>) n\<close> by auto
+  moreover have "\<sigma> \<in> Pow (M_i (V,C,\<epsilon>) (n-1))"
+    using \<open>\<sigma> \<in> \<Sigma>_i (V, C, \<epsilon>) n\<close> si by auto
+  hence "\<sigma> \<in> Pow (M_i (V,C,\<epsilon>) n)"
+    using Mi_monotonic
+    by (metis (full_types) PowD PowI Suc_eq_plus1 \<open>\<exists>n'. n = Suc n'\<close> diff_Suc_1 subset_iff)
+  ultimately have "\<sigma> \<union> {m} \<in> Pow (M_i (V,C,\<epsilon>) n)"
+    by blast
+
+  show "\<sigma> \<union> {m} \<in> \<Sigma>_i (V, C, \<epsilon>) (n + 1)"
+    using \<open>\<And>m'. m' \<in> \<sigma> \<Longrightarrow> justification m' \<subseteq> \<sigma> \<union> {m}\<close> \<open>\<sigma> \<union> {m} \<in> Pow (M_i (V, C, \<epsilon>) n)\<close> \<open>justification m \<subseteq> \<sigma> \<union> {m}\<close> by auto
+qed
+
+lemma (in Protocol) state_transition_by_immediately_next_message_at_n: "\<forall>\<sigma>\<in>\<Sigma>_i (V,C,\<epsilon>) n. \<forall>m\<in>M_i (V,C,\<epsilon>) n. immediately_next_message (\<sigma>,m) \<longrightarrow> \<sigma> \<union> {m} \<in> \<Sigma>_i (V,C,\<epsilon>) (n+1)"
+  apply (cases n)
+  apply auto[1]
+  using state_transition_by_immediately_next_message_induction
+  by (metis le_add1 plus_1_eq_Suc)
+
+lemma (in Protocol) state_differences_have_immediately_next_messages: 
+  "\<forall> \<sigma> \<in> \<Sigma>. \<forall> \<sigma>'\<in> \<Sigma>. is_future_state (\<sigma>', \<sigma>) \<and> \<sigma> \<noteq> \<sigma>' \<longrightarrow> (\<exists> m \<in> \<sigma>'-\<sigma>. immediately_next_message (\<sigma>, m))"
+  apply (simp add: immediately_next_message_def)
+  apply (rule, rule, rule)
+proof -
+  fix \<sigma> \<sigma>'
+  assume "\<sigma> \<in> \<Sigma>"
+  assume "\<sigma>' \<in> \<Sigma>"
+  assume "\<sigma> \<subseteq> \<sigma>' \<and> \<sigma> \<noteq> \<sigma>'"
+  show "\<exists> m \<in> \<sigma>' - \<sigma>. justification m \<subseteq> \<sigma>"
+  proof (rule ccontr)
+    assume "\<not> (\<exists> m \<in> \<sigma>' - \<sigma>. justification m \<subseteq> \<sigma>)"
+    have "\<forall> m \<in> \<sigma>' - \<sigma>. \<exists> m' \<in> justification m. m' \<in> \<sigma>' - \<sigma>"
+      using \<open>\<not> (\<exists>m\<in>\<sigma>' - \<sigma>. justification m \<subseteq> \<sigma>)\<close> \<open>\<sigma>' \<in> \<Sigma>\<close> state_is_in_pow_M_i by fastforce
+    then have "\<forall> m \<in> \<sigma>' - \<sigma>. \<exists> m' \<in> justification m. m' \<in> \<sigma>' - \<sigma> \<and> m \<noteq> m'"
+      using \<open>\<sigma>' \<in> \<Sigma>\<close> irreflexivity_of_justifications state_is_subset_of_M by fastforce 
+    show False
+      sorry
+  qed
+qed
+
+lemma (in Protocol) minimal_transition_implies_recieving_a_single_message :
+  "\<forall> \<sigma> \<sigma>'. \<sigma> \<in> \<Sigma>t \<and> \<sigma>' \<in> \<Sigma>t
+  \<longrightarrow> (\<sigma>, \<sigma>') \<in> minimal_transitions  \<longrightarrow> is_singleton (\<sigma>'- \<sigma>)"
+  sorry
+
+end
